<div class ="alert alert-success">
** Theorem 1 **
 <center>
If $\text{dom } f$ is a convex set and f is differentiable, then f is a convex function if and only if $[\nabla f(y)-\nabla f (x)]^T(y-x) \geq 0$</center>
 </div>

$\textbf{Proof:}$

$\textit{Necessity}$: If f is a convex function, then $\nabla f(x)^T(y-x)\leq f(y) -f(x)$, for any x and y. One could easily get the result. 

$\textit{Sufficiency}$:  First, we set $ g(t) = f[x+t(y-x)]$, with $t\in [0,1]$. Then $$\begin{array}{cl}
f(y) & = g(1) = g(0) + \int_0^1 g'(t) dt \\
     & = f(x) + \int_0^1 (y-x)^T \nabla f[x+t(y-x)] dt \\
     & = f(x) + \nabla f(x)^T(y-x) + \int_0^1 (y-x)^T [f[x+t(y-x)]  - \nabla f(x)] dt\\
     & \geq  f(x) + \nabla f(x)^T(y-x)\end{array}$$
     
     
---

 <div class ="alert alert-success">
** Theorem 2 **
<center> Suppose f is a convex function, and at some point $f(y) = f(x) + \nabla f (x)^T (y-x)\ \ $ or $\ \ [\nabla f(y)-\nabla f (x)]^T(y-x) = 0 $, then  $ f[ty+(1-t)x] =(1-t) f(x) + t f(y)$, for all  $0 \leq t \leq 1$</center>
 </div>
 

$\textbf{Proof:}$

As $$f(y) - f[x+ t(y-x)] \geq (1-t) \nabla f[x+ t(y-x)]^T(y-x)  $$ and $$ f[x+ t(y-x)] - f(x) \geq  t\nabla f (x)^T (y-x) $$ then one could derive that $$f(y) - f(x) \geq (1-t) \nabla f[x+ t(y-x)]^T(y-x)   +  t\nabla f (x)^T (y-x) $$.  
Substitute $f(y) = f(x) + \nabla f (x)^T (x)$ into the equation above, then
$$[\nabla f (x)  -\nabla f(x+ t(y-x))] ^T(y-x)\leq 0.$$  However, f is convex function, we also have that $$\{\nabla f (x)  -\nabla f[x+ t(y-x)]\} ^T(y-x)\geq 0$$

Then the left side of equation above must be 0.  Then $f[x+ t(y-x)]$ is a linear function of t, which leads to a fact that 
$$f[ty+(1-t)x] =(1-t) f(x) + t f(y)$$

A similar result could be conducted in the case that $\ \ [\nabla f(y)-\nabla f (x)]^T(y-x) = 0 $.

---
 <div class ="alert alert-success">
** Theorem 3 **
<center>If f is differentiable, then f is a strictly cenvex function if and only if $\nabla f(x)^T(y-x)< f(y) -f(x)$ or  $[\nabla f(y)-\nabla f (x)]^T(y-x) > 0 $</center>
 </div>
 
Remark: in the proof on not strictly convex function, by taking a limit, we achive the result. But in a strictly convex function, we need to pay attention that a strictly inequaltiy may become a equality under a limit. For example, even  $ 1-\frac{1}{n}<1$, but when take a limit we have 
$\underset{ n\to \infty} {\text{lim}}(1-\frac{1}{n}) =1 $.

$\textbf{Proof:}$

$\textit{Sufficiency}$: If $\nabla f(x)^T(y-x)=f(y) -f(x)$ or  $[\nabla f(y)-\nabla f (x)]^T(y-x) = 0 $, from the theorem 2, $ f[ty+(1-t)x] =(1-t) f(x) + t f(y)$, for all  $0 \leq t \leq 1$. Then f is not strictly convex.  

$\textit{Necessity}$: One could prove it as not strictly convex function's condition.
"
